Common/Blame.v
@@ -11,14 +11,8 @@ Definition extract_finite_trace (beh: program_behavior) : option trace :=
   | Goes_wrong t => Some t
   end.
 
-Definition who_is_in_control_after (e: event) : Component.id :=
-  match e with
-  | ECall _ _ _ C => C
-  | ERet _ _ C => C
-  end.
-
 Definition last_comp (t: trace) :=
-  last Component.main [seq who_is_in_control_after e | e <- t].
+  last Component.main [seq next_comp_of_event e | e <- t].
 
 Definition undef_in (t: trace) (iface: Program.interface) :=
   last_comp t \in domm iface.
