Source/GlobalEnv.v
@@ -7,11 +7,9 @@ Import Source.
 
 Record global_env : Type := mkGlobalEnv {
   genv_interface : Program.interface;
-  genv_procedures : NMap (NMap expr);
-  genv_buffers : NMap Block.id
+  genv_procedures : NMap (NMap expr)
 }.
 
 Definition prepare_global_env (p: program) : global_env :=
   {| genv_interface := prog_interface p;
-     genv_procedures := prog_procedures p;
-     genv_buffers := snd (prepare_buffers p) |}.
+     genv_procedures := prog_procedures p |}.
